Restructuring qTesla specification

qtesla/spec/Spec.QTesla.fst
@@ -1,169 +1,56 @@
 module Spec.QTesla
 
-open FStar.Mul
-open FStar.List.Tot.Base
+open FStar.List.Tot
 open FStar.Seq
-open FStar.Seq.Base
+open FStar.Math.Lemmas
+open FStar.Mul
+
 open Lib.IntTypes
 open Lib.Sequence
 open Lib.ByteSequence
 open Lib.RawIntTypes
-open FStar.Math.Lemmas
-open Spec.QTesla.Sorting
 
-open Spec.Keccak
-open Spec.Frodo.Keccak
+open Spec.SHA3
+open QTesla.Params
 
-type nonzero_nat = x:nat{x > 0}
+#reset-options "--z3rlimit 50 --max_fuel 0 --max_ifuel 1"
 
-// qTESLA-I
-(*
-let params_lambda:nat = 95 // security parameter
-let params_kappa:nat = 32 // output length of hash function in bytes (spec lists them in bits, so convert)
-let params_n:size_nat = 512 // Dimension
-let params_k:size_nat = 1       // #R-LWE samples (number of polynomials in e, t, a, etc)
-let params_q:int = 4205569 // modulus
-let params_h:nat = 30      // # of nonzero entries of output elements of Enc
-let params_Le:int = 1586   // bound on e_i for checkE
-let params_Ls:int = 1586   // bound on s for checkS
-let params_B:nat = 1048575 // interval the randomness is chosing from during signing
-let params_d:nat = 21      // number of rounded bits
-let params_bGenA:int = 19  // number of blocks requested to SHAKE128 for GenA
+(** qTesla often uses [pos] as a variable name, so we define a transparent synonym *)
+unfold let positive = pos
 
-let params_rateXOF = 168
-let params_xof = shake128        // extendable output function used in PRF1: use shake128 or shake256 depending on parameters chosen
-let params_hash_shake = shake128 // hash function used in hash H: use shake128 or shake256 depending on parameters chosen
-
-// See the GenerateNTTConstants-Magma.txt script for computing these five
-// constants used in NTT.
-let computed_phi = 3768668
-let computed_omega = 118029
-let computed_phi_inv = 3764481
-let computed_omega_inv = 590666
-let computed_n_inv = 4197355
+(** 
+* Computes ceil(log2 n) using the equation
+* ceil(log2 n) = floor(log2 (2 * n - 1)
 *)
-// end qTESLA-I parameters
+val log2: pos -> nat
+let log2 n =
+  let rec floor_log2 (n:pos) : nat =
+    if n = 1 then 0
+    else 1 + floor_log2 (n / 2)
+  in floor_log2 (2 * n - 1)
 
-// qTESLA-III-speed
-(*
-let params_lambda:nat = 160 // security parameter
-let params_kappa:nat = 32 // output length of hash function in bytes (spec lists them in bits, so convert)
-let params_n:size_nat = 1024 // Dimension
-let params_k:size_nat = 1       // #R-LWE samples (number of polynomials in e, t, a, etc)
-let params_q:int = 8404993 // modulus
-let params_h:nat = 48      // # of nonzero entries of output elements of Enc
-let params_Le:int = 1147   // bound on e_i for checkE
-let params_Ls:int = 1233   // bound on s for checkS
-let params_B:nat = 2097151 // interval the randomness is chosing from during signing
-let params_d:nat = 22      // number of rounded bits
-let params_bGenA:int = 38  // number of blocks requested to SHAKE128 for GenA
+(** Computes ceil(a / b) *)
+val ceil_div: nat -> pos -> nat
+let ceil_div a b = if a % b = 0 then a / b else 1 + a / b
 
-let params_rateXOF = 168
-let params_xof = shake128        // extendable output function used in PRF1: use shake128 or shake256 depending on parameters chosen
-let params_hash_shake = shake128 // hash function used in hash H: use shake128 or shake256 depending on parameters chosen
+(** ceil(log_2 q) *)
+unfold let computed_ceil_log_q = normalize_term (log2 params_q)
 
-// See the GenerateNTTConstants-Magma.txt script for computing these five
-// constants used in NTT.
-let computed_phi = 5216957
-let computed_omega = 3851906
-let computed_phi_inv = 4276303
-let computed_omega_inv = 7267723
-let computed_n_inv = 8396785
+(** 
+* ceil((log_2 q) / 8)
+* Uses the equation ceil(a / b) = ceil(ceil(a) / b) 
 *)
-// end qTESLA-III-speed parameters
+unfold let computed_b = normalize_term (ceil_div (log2 params_q) 8)
 
-// qTESLA-III-size
-(*
-let params_lambda:nat = 160 // security parameter
-let params_kappa:nat = 32 // output length of hash function in bytes (spec lists them in bits, so convert)
-let params_n:size_nat = 1024 // Dimension
-let params_k:size_nat = 1       // #R-LWE samples (number of polynomials in e, t, a, etc)
-let params_q:int = 4206593 // modulus
-let params_h:nat = 48      // # of nonzero entries of output elements of Enc
-let params_Le:int = 910    // bound on e_i for checkE
-let params_Ls:int = 910    // bound on s for checkS
-let params_B:nat = 1048575 // interval the randomness is chosing from during signing
-let params_d:nat = 21      // number of rounded bits
-let params_bGenA:int = 38  // number of blocks requested to SHAKE128 for GenA
+(** ceil(((log_2 B) + 1) / 8) *)
+unfold let computed_ySampler_b = normalize_term (ceil_div (log2 params_B + 1) 8)
+  
+(** ceil(log_2 B) + 1 *)
+unfold let computed_ySampler_modulus = normalize_term (log2 params_B + 1)
 
-let params_rateXOF = 168
-let params_xof = shake128        // extendable output function used in PRF1: use shake128 or shake256 depending on parameters chosen
-let params_hash_shake = shake128 // hash function used in hash H: use shake128 or shake256 depending on parameters chosen
+/// Polynomial ring
 
-// See the GenerateNTTConstants-Magma.txt script for computing these five
-// constants used in NTT.
-let computed_phi = 3999147
-let computed_omega = 396526
-let computed_phi_inv = 1974815
-let computed_omega_inv = 3979855
-let computed_n_inv = 4202485
-*)
-// end qTESLA-III-size parameters
-
-// qTESLA-p-I
-(*
-let params_lambda:nat = 95 // security parameter
-let params_kappa:nat = 32 // output length of hash function in bytes (spec lists them in bits, so convert)
-let params_n:size_nat = 1024 // Dimension
-let params_k:size_nat = 4       // #R-LWE samples (number of polynomials in e, t, a, etc)
-let params_q:int = 485978113 // modulus
-let params_h:nat = 25      // # of nonzero entries of output elements of Enc
-let params_Le:int = 554    // bound on e_i for checkE
-let params_Ls:int = 554    // bound on s for checkS
-let params_B:nat = 2097151 // interval the randomness is chosing from during signing
-let params_d:nat = 22      // number of rounded bits
-let params_bGenA:int = 108 // number of blocks requested to SHAKE128 for GenA
-
-let params_rateXOF = 168
-let params_xof = shake128        // extendable output function used in PRF1: use shake128 or shake256 depending on parameters chosen
-let params_hash_shake = shake128 // hash function used in hash H: use shake128 or shake256 depending on parameters chosen
-
-// See the GenerateNTTConstants-Magma.txt script for computing these five
-// constants used in NTT.
-let computed_phi = 250428822
-let computed_omega = 483976553
-let computed_phi_inv = 195194787
-let computed_omega_inv = 67220789
-let computed_n_inv = 485503525
-*)
-// end qTESLA-p-I parameters
-
-// qTESLA-p-III
-
-let params_lambda:nat = 160 // security parameter
-let params_kappa:nat = 32 // output length of hash function in bytes (spec lists them in bits, so convert)
-let params_n:size_nat = 2048 // Dimension
-let params_k:size_nat = 5       // #R-LWE samples (number of polynomials in e, t, a, etc)
-let params_q:int = 1129725953 // modulus
-let params_h:nat = 40      // # of nonzero entries of output elements of Enc
-let params_Le:int = 901    // bound on e_i for checkE
-let params_Ls:int = 901    // bound on s for checkS
-let params_B:nat = 8388607 // interval the randomness is chosing from during signing
-let params_d:nat = 24      // number of rounded bits
-let params_bGenA:int = 180 // number of blocks requested to SHAKE128 for GenA
-
-let params_rateXOF = 168
-let params_xof = shake128        // extendable output function used in PRF1: use shake128 or shake256 depending on parameters chosen
-let params_hash_shake = shake128 // hash function used in hash H: use shake128 or shake256 depending on parameters chosen
-
-// See the GenerateNTTConstants-Magma.txt script for computing these five
-// constants used in NTT.
-let computed_phi = 752833504
-let computed_omega = 905348506
-let computed_phi_inv = 500168718
-let computed_omega_inv = 224686349
-let computed_n_inv = 1129174329
-
-// end qTESLA-p-III parameters
-
-// End of parameter settings.
-let field_t = x:int{x > -params_q /\ x < params_q}
-
-let computed_ceil_log_q:nat = 23 // Computed: ceil(log_2 q)
-let computed_b:size_nat = 3           // Computed: ceil((log_2 q)/8)
-
-let computed_ySampler_b:nat = 3  // Computed: ceil(((log_2 B) + 1)/8), B = 2^20-1
-let computed_ySampler_modulus:nat = 21  // Computed: ceil(log_2 B) + 1
+let field_t = x:int{-params_q < x /\ x < params_q}
 
 // Single polynomial in \mathcal{R}_q/<x^n+1>
 let poly_t = Seq.lseq field_t params_n
@@ -171,9 +58,9 @@ let poly_t = Seq.lseq field_t params_n
 // Set of k polynomials in \mathcal{R}/(x^n+1)
 let polys_t = Seq.lseq poly_t params_k 
 
-let qtesla_sk = tuple4 poly_t polys_t (lbytes params_kappa) (lbytes params_kappa)
-let qtesla_pk = tuple2 (lbytes params_kappa) polys_t
-let qtesla_sig = tuple2 poly_t (lbytes params_kappa)
+let qtesla_sk = poly_t & polys_t & (lbytes params_kappa) & (lbytes params_kappa)
+let qtesla_pk = (lbytes params_kappa) & polys_t
+let qtesla_sig = poly_t & (lbytes params_kappa)
 
 val to_lseq: #a:Type0 -> s:Seq.seq a -> l:Seq.lseq a (Seq.length s){l == s}
 let to_lseq #a s = s
@@ -186,19 +73,19 @@ let create_polys : polys_t = to_lseq (Seq.create params_k create_poly)
 (* A lot of this polynomial ring math taken from the Kyber spec *)
 
 (* a + b (mod q); a, b \in Z_q *)
-val fadd: a:field_t -> b:field_t -> Tot field_t
+val fadd: field_t -> field_t -> field_t
 let fadd a b = (a + b) % params_q
 
 (* a - b (mod q); a, b \in Z_q *)
-val fsub: a:field_t -> b:field_t -> Tot field_t
+val fsub: field_t -> field_t -> field_t
 let fsub a b = (params_q + a - b) % params_q
 
 (* a * b (mod q); a, b \in Z_q *)
-val fmul: a:field_t -> b:field_t -> Tot field_t
+val fmul: field_t -> field_t -> field_t
 let fmul a b = (a * b) % params_q
 
 (* a ^ b (mod q); a, b \in Z_q *)
-val fexp: e:field_t -> n:nat -> Tot field_t (decreases n)
+val fexp: field_t -> n:nat -> Tot field_t (decreases n)
 let rec fexp e n =
   if n = 0 then 1
   else if n = 1 then e
@@ -211,37 +98,43 @@ let ( ++ ) = fadd
 let ( -- ) = fsub
 let ( ^^ ) = fexp
 
-val map2_step: res:poly_t -> f:(field_t -> field_t -> Tot field_t) -> x:poly_t -> y:poly_t -> i:size_nat{i <= params_n} -> Tot poly_t (decreases (params_n - i))
+val map2_step: 
+    poly_t 
+  -> (field_t -> field_t -> field_t) 
+  -> poly_t 
+  -> poly_t 
+  -> i:size_nat{i <= params_n} 
+  -> Tot poly_t (decreases (params_n - i))
 let rec map2_step res f x y i =
-  if (i = Seq.length x)
+  if i = Seq.length x
   then res
   else let res = Seq.upd res i (f (Seq.index x i) (Seq.index y i)) in
        map2_step res f x y (i + 1)
 
-val map2: f:(field_t -> field_t -> Tot field_t) -> x:poly_t -> y:poly_t -> Tot poly_t
+val map2: (field_t -> field_t -> field_t) -> poly_t -> poly_t -> poly_t
 let map2 f x y =
   let res = create_poly in
   map2_step res f x y 0
 
 (* a + b (mod q); a, b \in \mathcal{R}_q/<x^n+1> *)
-val poly_add: a:poly_t -> b:poly_t -> Tot poly_t
+val poly_add: poly_t -> poly_t -> poly_t
 let poly_add a b = map2 fadd a b
 
 (* a - b (mod q); a, b \in \mathcal{R}_q/<x^n+1> *)
-val poly_sub: a:poly_t -> b:poly_t -> Tot poly_t
+val poly_sub: poly_t -> poly_t -> poly_t
 let poly_sub a b = map2 fsub a b
 
 (* a o b (mod q) [pointwise coefficient multiplication]; a, b \in \mathcal{R}_q/<x^n+1> *)
-val poly_pointwise_mul: a:poly_t -> b:poly_t -> Tot poly_t
+val poly_pointwise_mul: poly_t -> poly_t -> poly_t
 let poly_pointwise_mul a b = map2 fmul a b
 
-val ntt: p:poly_t -> Tot poly_t
+val ntt: poly_t -> poly_t
 let ntt p =
   let np = p in
   repeati params_k (fun i (np:poly_t) ->
 		 Seq.upd np i (repeati params_k (fun j x -> x ++ ((computed_phi ^^ j) ** (Seq.index p j) ** (computed_omega ^^ (i * j)))) 0)) np
 
-val inv_ntt: p:poly_t -> Tot poly_t
+val inv_ntt: poly_t -> poly_t
 let inv_ntt p =
   let np = p in
   repeati params_n (fun i (np:poly_t) ->
@@ -249,104 +142,136 @@ let inv_ntt p =
 
 (* a * b (mod q); a, b \in \mathcal{R}_q/<x^n+1> *)
 (* qTESLA specific assumption: a is always in NTT form, and b is always in standard form. Use poly_mul for two polynomials in standard form. *)
-val poly_ntt_mul: a:poly_t -> b:poly_t -> Tot poly_t
+val poly_ntt_mul: poly_t -> poly_t -> poly_t
 let poly_ntt_mul a b =
   inv_ntt (a `poly_pointwise_mul` (ntt b))
 
 (* a * b (mod q); a, b \in \mathcal{R}_q/<x^n+1> *)
 (* a, b in standard form *)
-val poly_mul: a:poly_t -> b:poly_t -> Tot poly_t
+val poly_mul: poly_t -> poly_t -> poly_t
 let poly_mul a b =
   inv_ntt ((ntt a) `poly_pointwise_mul` (ntt b))
   
-(* End of polynomial ring math *)
+/// End of polynomial ring math
 
-val sum: l:list int -> Tot int
+val sum: list int -> Tot int
 let rec sum l =
   match l with
   | [] -> 0
   | hd :: tl -> hd + sum tl
 
-val sort_coefficients: p: poly_t -> Tot poly_t
-let sort_coefficients p = sort_lseq (<=) p
+val sort_coefficients: poly_t -> poly_t
+let sort_coefficients p = Seq.sort_lseq (<=) p
   
-val poly_max_sum_helper: sorted:poly_t -> h:nat{h < Seq.length sorted} -> Tot int
+val poly_max_sum_helper: sorted:poly_t -> h:nat{h < Seq.length sorted} -> int
 let rec poly_max_sum_helper sorted h =
   let res = Seq.index sorted h in
     if h = 0
     then res
     else res + poly_max_sum_helper sorted (h - 1)
 
-val poly_max_sum: p:poly_t -> h:nat{h < Seq.length p} -> Tot int
+val poly_max_sum: p:poly_t -> h:nat{h < Seq.length p} -> int
 let poly_max_sum p h =
   let sorted = sort_coefficients p in
   perm_len sorted p;
   poly_max_sum_helper sorted h
   
 // Sum the h largest coefficients of s, and return true if bounded by L_s
-val checkS: s:poly_t -> Tot bool
+val checkS: poly_t -> bool
 let checkS s = poly_max_sum s params_h <= params_Ls
 
 // Sum the h largest coefficients of e_i, and return true if bounded by L_e
-val checkE: e:poly_t -> Tot bool
+val checkE: poly_t -> bool
 let checkE e = poly_max_sum e params_h <= params_Le
 
 // Given an input pre-seed of \kappa bytes, return a buffer of (\kappa * ((k+3)/8)) bytes extended by the XOF
-val prf1: preseed:lbytes params_kappa -> lbytes (params_kappa * (params_k+3))
+val prf1: lbytes params_kappa -> lbytes (params_kappa * (params_k+3))
 let prf1 preseed = params_xof params_kappa preseed (params_kappa * (params_k+3))
 
-val prf2: #mLen:size_nat{mLen < maxint SIZE - 2 * params_kappa} -> seedY: (lbytes params_kappa) -> r: (lbytes params_kappa) -> m: (lbytes mLen) -> Tot (lbytes params_kappa)
+val prf2: 
+    #mLen:size_nat{mLen < maxint SIZE - 2 * params_kappa} 
+  -> seedY:lbytes params_kappa 
+  -> r:lbytes params_kappa 
+  -> m:lbytes mLen 
+  -> lbytes params_kappa
 let prf2 #mLen seedY r m =
   let concatenation = concat (concat seedY r) m in
   params_xof (length concatenation) concatenation params_kappa
 
-val genA_getC: cBuf: bytes -> cPos: size_nat{(cPos+1) * computed_b <= length cBuf} -> Tot size_nat
+val genA_getC: 
+    cBuf:bytes 
+  -> cPos:size_nat{(cPos+1) * computed_b <= length cBuf} 
+  -> size_nat
 let genA_getC cBuf cPos = 
   let subbuffer = slice (to_lbytes cBuf) (cPos * computed_b) ((cPos+1) * computed_b) in
   nat_from_bytes_le subbuffer
 
-val genA_updateA: a:polys_t -> i:nat{i < params_k * params_n} -> newVal:field_t -> Tot polys_t
+val genA_updateA: polys_t -> i:nat{i < params_k * params_n} -> field_t -> polys_t
 let genA_updateA a i newVal =
   let polyNum = i / params_n in
   let coefNum = i - params_n * polyNum in
   let ax = Seq.index a polyNum in
   let axy = Seq.upd ax coefNum newVal in
-    Seq.upd a polyNum ax
+  Seq.upd a polyNum ax
 
 (* We have a strange termination condition with this while loop. If cSHAKE was completely broken, it could theoretically return an array of bytes such that every b-byte subarray interpreted as a natural number was greater than equal to the modulus parameter q. If it kept returning arrays like this, the function could theoretically loop infinitely. Of course this won't happen. It may be possible to prove something like "there is guaranteed to exist at least one element in the output array < q" but without even knowing what is provable about hash functions the F* experts thought this was difficult.
 
 So at their suggestion this code takes a different approach: We define the function to always terminate but with the possibility of failure, and then assume the existence of an "oracle" function that somehow tells us that if we end up calling cSHAKE a certain number of times, we're guaranteed to succeed. This is what the "fuel" parameter in genA_while and the definition of genA_oracle below it are all about. *)
 
-val genA_while: #seedALen:size_nat -> seedA: lbytes seedALen -> cBuf: bytes{length cBuf >= 2} -> s:uint16 -> a:polys_t -> pos: size_nat{(pos+1) * computed_b <= length cBuf} -> bPrime:size_nat{bPrime >= 1 /\ params_rateXOF * bPrime = length cBuf} -> i:nat -> fuel:nat -> Tot (option polys_t) (decreases %[(params_k * params_n - i); fuel])
+val genA_while: 
+    #seedALen:size_nat 
+  -> seedA: lbytes seedALen 
+  -> cBuf: bytes{length cBuf >= 2} 
+  -> s:uint16 
+  -> a:polys_t 
+  -> pos: size_nat{(pos+1) * computed_b <= length cBuf} 
+  -> bPrime:size_nat{bPrime >= 1 /\ params_rateXOF * bPrime = length cBuf} 
+  -> i:nat 
+  -> fuel:nat 
+  -> Tot (option polys_t) (decreases %[(params_k * params_n - i); fuel])
 let rec genA_while #seedALen seedA cBuf s a pos bPrime i fuel =
-  if fuel = 0 then None else
-  if i < params_k * params_n
-    then let s, pos, bPrime, cBuf =
-      if pos > ((params_rateXOF * bPrime) / computed_b) - 4
-      then let s, pos, bPrime = (add_mod s (u16 1)), 0, 1 in
-           let cBuf = cshake128_frodo seedALen seedA s (params_rateXOF * bPrime) in
-	   s, pos, bPrime, cBuf
-      else s, pos, bPrime, cBuf in
+  assert_norm (0 < computed_b /\ computed_b < 10);
+  if fuel = 0 then None 
+  else if i < params_k * params_n
+  then 
+    let s, pos, bPrime, cBuf =
+      if pos > ((params_rateXOF * bPrime) / computed_b) - 4 then 
+        let s, pos, bPrime = add_mod s (u16 1), 0, 1 in
+        let cBuf = cshake128_frodo seedALen seedA s (params_rateXOF * bPrime) in
+        s, pos, bPrime, cBuf
+      else 
+        s, pos, bPrime, cBuf 
+    in
     let c_pos = genA_getC cBuf pos in
       let a, i, fuel =
         let c_pos_mod = c_pos % (pow2 computed_ceil_log_q) in
 	if params_q > c_pos_mod
 	then genA_updateA a i c_pos_mod, i + 1, fuel
-	else a, i, fuel - 1 in
-      let pos = pos + 1 in
-      genA_while #seedALen seedA cBuf s a pos bPrime i fuel
-    else Some a
+	else a, i, fuel - 1 
+      in
+      genA_while #seedALen seedA cBuf s a (pos + 1) bPrime i fuel
+  else Some a
 
-assume val genA_oracle: #seedALen:size_nat -> seedA: lbytes seedALen -> cBuf: bytes -> s:uint16 -> a:polys_t -> pos: size_nat{(pos+1) * computed_b < length cBuf} -> bPrime:size_nat{bPrime >= 1 /\ params_rateXOF * bPrime = length cBuf} -> i:nat -> Tot (fuel:nat{Some? (genA_while #seedALen seedA cBuf s a pos bPrime i fuel)})
+assume 
+val genA_oracle: 
+    #seedALen:size_nat 
+  -> seedA: lbytes seedALen 
+  -> cBuf: bytes 
+  -> s:uint16 
+  -> a:polys_t 
+  -> pos: size_nat{(pos+1) * computed_b < length cBuf} 
+  -> bPrime:size_nat{bPrime >= 1 /\ params_rateXOF * bPrime = length cBuf} 
+  -> i:nat 
+  -> Tot (fuel:nat{Some? (genA_while #seedALen seedA cBuf s a pos bPrime i fuel)})
   
-val genA: #seedALen: size_nat -> seedA: lbytes seedALen -> Tot polys_t
+val genA: #seedALen:size_nat -> seedA:lbytes seedALen -> polys_t
 let genA #seedALen seedA =
   let bPrime = params_bGenA in
   let cBuf = cshake128_frodo seedALen seedA (u16 0) (params_rateXOF * bPrime) in
   let i = 0 in
   let pos = 0 in
   let a = create_polys in
-  let fuel:nat = genA_oracle seedA cBuf (u16 0) a pos bPrime i in
+  let fuel = genA_oracle seedA cBuf (u16 0) a pos bPrime i in
   let res = genA_while seedA cBuf (u16 0) a pos bPrime i fuel in
   Some?.v res
 
@@ -354,59 +279,87 @@ let genA #seedALen seedA =
 // gaussSampler is assumed because it has floating point math we can't
 // yet model in F*. random_bytes is assumed because it needs to come from
 // an underlying system source.
-assume val gaussSampler: rand: (lbytes params_kappa) -> nonce: nat{nonce > 0} -> Tot poly_t
-assume val random_bytes: n: size_nat -> Tot (lbytes n)
+assume val gaussSampler: rand: (lbytes params_kappa) -> nonce: nat{nonce > 0} -> poly_t
+
+assume val random_bytes: n: size_nat -> lbytes n
 
 // Termination is probabilistic due to the need to get the right sort
 // of output from the sampler, and so we use the fuel method again.
-val keygen_sample_while: seed: (lbytes params_kappa) -> nonce: nonzero_nat -> checkFn: (poly_t -> Tot bool) -> fuel: nat -> Tot (option (tuple2 poly_t nonzero_nat)) (decreases fuel)
+val keygen_sample_while: 
+    seed: lbytes params_kappa 
+  -> nonce: positive 
+  -> checkFn: (poly_t -> bool) 
+  -> fuel: nat 
+  -> Tot (option (tuple2 poly_t positive)) (decreases fuel)
 let rec keygen_sample_while seed nonce checkFn fuel =
   if fuel = 0 then None else
   let s = gaussSampler seed nonce in
   if checkFn s then Some (s, nonce)
                else keygen_sample_while seed (nonce + 1) checkFn (fuel - 1)
 
-assume val keygen_sample_oracle: seed: (lbytes params_kappa) -> nonce: nat{nonce > 0} -> checkFn: (poly_t -> Tot bool) -> Tot (fuel:nat{Some? (keygen_sample_while seed nonce checkFn fuel)})
+assume val keygen_sample_oracle: 
+    seed: lbytes params_kappa
+  -> nonce: nat{nonce > 0} 
+  -> checkFn: (poly_t -> bool) 
+  -> Tot (fuel:nat{Some? (keygen_sample_while seed nonce checkFn fuel)})
 
-let keygen_sampleS_while seedS nonce = Some?.v (keygen_sample_while seedS nonce checkS (keygen_sample_oracle seedS nonce checkS))
-let keygen_sampleE_while seedE nonce = Some?.v (keygen_sample_while seedE nonce checkE (keygen_sample_oracle seedE nonce checkE))
+let keygen_sampleS_while seedS nonce = 
+  Some?.v (keygen_sample_while seedS nonce checkS (keygen_sample_oracle seedS nonce checkS))
 
-#reset-options "--z3rlimit 50 --max_fuel 0"
-val keygen_sampleE_step: seedE:(lbytes (params_kappa * params_k)) -> nonce:nonzero_nat -> e:polys_t -> i:size_nat{i <= Seq.length e} -> Tot (tuple2 polys_t nonzero_nat) (decreases (Seq.length e - i))
+let keygen_sampleE_while seedE nonce = 
+  Some?.v (keygen_sample_while seedE nonce checkE (keygen_sample_oracle seedE nonce checkE))
+
+val keygen_sampleE_step: 
+    seedE:lbytes (params_kappa * params_k) 
+  -> nonce:positive 
+  -> e:polys_t 
+  -> i:size_nat{i <= Seq.length e} 
+  -> Tot (tuple2 polys_t positive) (decreases (Seq.length e - i))
 let rec keygen_sampleE_step seedE nonce e i =
-  if i = Seq.length e then e, nonce
-		      else let seedEi = Lib.Sequence.sub seedE (i * params_kappa) params_kappa in
-		           let ei, nonce = keygen_sampleE_while seedEi nonce in
-		           let e = Seq.upd e i ei in
-			   keygen_sampleE_step seedE nonce e (i + 1)
+  if i = Seq.length e then 
+    e, nonce
+  else 
+    let seedEi = Lib.Sequence.sub seedE (i * params_kappa) params_kappa in
+    let ei, nonce = keygen_sampleE_while seedEi nonce in
+    let e = Seq.upd e i ei in
+    keygen_sampleE_step seedE nonce e (i + 1)
 
-val keygen_sampleE: seedE:(lbytes (params_kappa * params_k)) -> nonce:nonzero_nat -> Tot (tuple2 polys_t nonzero_nat)
+val keygen_sampleE: 
+    seedE:(lbytes (params_kappa * params_k)) 
+  -> nonce:positive 
+  -> tuple2 polys_t positive
 let keygen_sampleE seedE nonce = 
   let e = create_polys in
   keygen_sampleE_step seedE nonce e 0
 
-val poly_mod: f:poly_t -> n:nat{n >= 2 /\ n <= params_q} -> Tot poly_t
+val poly_mod: f:poly_t -> n:nat{2 <= n /\ n <= params_q} -> poly_t
 let poly_mod f n =
   repeati (Seq.length f)
   (fun i (f:poly_t) ->
     let fi = (Seq.index f i) % n in
     Seq.upd f i fi) f
 
-val keygen_computeT_step: a:polys_t -> s:poly_t -> e:polys_t -> t:polys_t -> i:size_nat{i <= Seq.length a} -> Tot polys_t (decreases (Seq.length a - i))
+val keygen_computeT_step: 
+     a:polys_t 
+   -> s:poly_t 
+   -> e:polys_t 
+   -> t:polys_t 
+   -> i:size_nat{i <= Seq.length a} 
+   -> Tot polys_t (decreases (Seq.length a - i))
 let rec keygen_computeT_step a s e t i =
   if i = Seq.length a then t
-    else // Remember, a is always in NTT form; other polys in standard form
-         let ti = (((Seq.index a i) `poly_ntt_mul` s) `poly_add` (Seq.index e i)) `poly_mod` params_q in
-	 let t = Seq.upd t i ti in
-	 keygen_computeT_step a s e t (i + 1)
+  else // Remember, a is always in NTT form; other polys in standard form
+    let ti = (((Seq.index a i) `poly_ntt_mul` s) `poly_add` (Seq.index e i)) `poly_mod` params_q in
+    let t = Seq.upd t i ti in
+    keygen_computeT_step a s e t (i + 1)
 
-val keygen_computeT: a:polys_t -> s:poly_t -> e:polys_t -> Tot polys_t
+val keygen_computeT: a:polys_t -> s:poly_t -> e:polys_t -> polys_t
 let keygen_computeT a s e =
   let t = create_polys in
   keygen_computeT_step a s e t 0
 
-//val qTesla_keygen: Tot (tuple2 qtesla_sk qtesla_pk)
-let qTesla_keygen : tuple2 qtesla_sk qtesla_pk =
+val qTesla_keygen: qtesla_sk & qtesla_pk
+let qTesla_keygen =
   let preseed = random_bytes params_kappa in
   let seedbuf = prf1 preseed in
   let seedS_begin = 0 in
@@ -436,7 +389,16 @@ let qTesla_keygen : tuple2 qtesla_sk qtesla_pk =
 
 let ySampler_XOF = cshake128_frodo
 
-val ySampler_while: rand: lbytes params_kappa -> cBuf: bytes -> pos: size_nat -> nPrime: size_nat{computed_ySampler_b * nPrime <= max_size_t /\ computed_ySampler_b * nPrime = length cBuf} -> sPrime: uint16 -> i: size_nat{i <= params_n} -> y: poly_t -> fuel:nat -> Tot (option poly_t) (decreases %[(params_n - i); fuel])
+val ySampler_while: 
+    rand: lbytes params_kappa 
+  -> cBuf: bytes 
+  -> p: size_nat 
+  -> nPrime: size_nat{computed_ySampler_b * nPrime <= max_size_t /\ computed_ySampler_b * nPrime = length cBuf} 
+  -> sPrime: uint16 
+  -> i: size_nat{i <= params_n} 
+  -> y: poly_t 
+  -> fuel:nat 
+  -> Tot (option poly_t) (decreases %[(params_n - i); fuel])
 let rec ySampler_while rand cBuf pos nPrime sPrime i y fuel =
   if fuel = 0 then None else
   let b = computed_ySampler_b in
@@ -457,9 +419,18 @@ let rec ySampler_while rand cBuf pos nPrime sPrime i y fuel =
     ySampler_while rand cBuf pos nPrime sPrime i y fuel
   else Some y
 
-assume val ySampler_oracle: rand: lbytes params_kappa -> cBuf: bytes -> pos: size_nat -> nPrime: size_nat{computed_ySampler_b * nPrime <= max_size_t /\ computed_ySampler_b * nPrime = length cBuf} -> sPrime: uint16 -> i: size_nat{i <= params_n} -> y: poly_t -> Tot (fuel:nat{Some? (ySampler_while rand cBuf pos nPrime sPrime i y fuel)})
+assume 
+val ySampler_oracle: 
+    rand: lbytes params_kappa 
+  -> cBuf: bytes 
+  -> pos: size_nat 
+  -> nPrime: size_nat{computed_ySampler_b * nPrime <= max_size_t /\ computed_ySampler_b * nPrime = length cBuf} 
+  -> sPrime: uint16 
+  -> i: size_nat{i <= params_n} 
+  -> y: poly_t 
+  -> Tot (fuel:nat{Some? (ySampler_while rand cBuf pos nPrime sPrime i y fuel)})
 
-val ySampler: rand: lbytes params_kappa -> nonce: uint16 -> Tot poly_t
+val ySampler: lbytes params_kappa -> uint16 -> poly_t
 let ySampler rand nonce =
   let b = computed_ySampler_b in
   let y = create_poly in
@@ -469,8 +440,11 @@ let ySampler rand nonce =
   let fuel = ySampler_oracle rand cBuf pos nPrime sPrime i y in
   Some?.v (ySampler_while rand cBuf pos nPrime sPrime i y fuel)
 
-#reset-options "--z3rlimit 50 --max_fuel 0"
-val hashH: #mlen: size_nat{params_k * params_n + mlen <= max_size_t} -> v: polys_t -> m: lbytes mlen -> Tot (lbytes params_kappa)
+val hashH: 
+    #mlen: size_nat{params_k * params_n + mlen <= max_size_t} 
+  -> polys_t 
+  -> lbytes mlen 
+  -> lbytes params_kappa
 let hashH #mlen v m =
   let w = Lib.Sequence.create (params_k * params_n + mlen) (u8 0) in
   let w = repeati params_k
@@ -486,8 +460,7 @@ let hashH #mlen v m =
 				     else val_ in
                let wiInt = (vij - val_) / (pow2 params_d) in
 	       (* TODO: Patrick tells us the above math guarantees wiInt is < 2^8. We should prove this properly. Assume it for now. *)
-	       assume (wiInt >= 0);
-	       assume (wiInt < maxint U8);
+	       assume (0 <= wiInt /\ wiInt < maxint U8);
 	       let wi = u8 wiInt in
 	       w.[i * params_n + j] <- wi
       ) w
@@ -500,13 +473,23 @@ let hashH #mlen v m =
 let signlist_elt = x:int{x = -1 \/ x == 1}
 let signlist_t = Seq.lseq signlist_elt params_h
 
-val enc_while_getR: #rLen:size_nat -> rBuf: (lbytes rLen) -> i:nat{i < rLen} -> Tot (x:nat{x < 256})
+val enc_while_getR: #rLen:size_nat -> rBuf:lbytes rLen -> i:nat{i < rLen} -> x:nat{x < 256}
 let enc_while_getR #rLen rBuf i =
   let byte = slice rBuf i (i+1) in
   nat_from_bytes_le byte
 
 (* pos_list and sign_list aren't returned by this function in the spec, although they are used in the implementation. We compute them here for consistency but only return c. *)
-val enc_while: cPrime: (lbytes params_kappa) -> rBuf: (lbytes params_rateXOF) -> pos_list: (Seq.lseq int params_h) -> sign_list: signlist_t -> cnt: size_nat -> c: poly_t -> s:uint16 -> i: size_nat -> fuel:nat -> Tot (option poly_t) (decreases %[(params_h - i); fuel])
+val enc_while: 
+    cPrime:lbytes params_kappa
+  -> rBuf:lbytes params_rateXOF
+  -> pos_list: Seq.lseq int params_h
+  -> sign_list: signlist_t 
+  -> cnt: size_nat 
+  -> c: poly_t 
+  -> s:uint16 
+  -> i: size_nat 
+  -> fuel:nat 
+  -> Tot (option poly_t) (decreases %[(params_h - i); fuel])
 let rec enc_while cPrime rBuf pos_list sign_list cnt c s i fuel =
   if fuel = 0 then None else
   if i < params_h then 
@@ -530,24 +513,34 @@ let rec enc_while cPrime rBuf pos_list sign_list cnt c s i fuel =
   enc_while cPrime rBuf pos_list sign_list cnt c s i fuel
   else Some c
 	       
-assume val enc_oracle: cPrime: (lbytes params_kappa) -> rBuf: (lbytes params_rateXOF) -> pos_list: (Seq.lseq int params_h) -> sign_list: signlist_t -> cnt: size_nat{cnt < params_rateXOF - 2} -> c: poly_t -> s:uint16 -> i: size_nat -> Tot (fuel:nat{Some? (enc_while cPrime rBuf pos_list sign_list cnt c s i fuel)})
+assume 
+val enc_oracle: 
+    cPrime: (lbytes params_kappa) 
+  -> rBuf: (lbytes params_rateXOF) 
+  -> pos_list: (Seq.lseq int params_h) 
+  -> sign_list: signlist_t 
+  -> cnt: size_nat{cnt < params_rateXOF - 2} 
+  -> c: poly_t 
+  -> s:uint16 
+  -> i: size_nat 
+  -> Tot (fuel:nat{Some? (enc_while cPrime rBuf pos_list sign_list cnt c s i fuel)})
 
-val enc: cPrime: (lbytes params_kappa) -> Tot poly_t
+val enc: lbytes params_kappa -> poly_t
 let enc cPrime =
-  let s = (u16 0) in
+  let s = u16 0 in
   let cnt = 0 in
   let rBuf = cshake128_frodo params_kappa cPrime s params_rateXOF in
   let i = 0 in
   let c:poly_t = create_poly in
-  let pos_list:(Seq.lseq int params_h) = Seq.create params_h 0 in
-  let sign_list:signlist_t = Seq.create params_h 1 in 
-  let fuel:nat = enc_oracle cPrime rBuf pos_list sign_list cnt c s i in
+  let pos_list: Seq.lseq int params_h = Seq.create params_h 0 in
+  let sign_list: signlist_t = Seq.create params_h 1 in 
+  let fuel = enc_oracle cPrime rBuf pos_list sign_list cnt c s i in
   let res = enc_while cPrime rBuf pos_list sign_list cnt c s i fuel in
   Some?.v res
 
-val mod_pm: a:int -> n:nat{n >= 2} -> Tot (x:int{x >= -(n/2) /\ x <= n/2})
+val mod_pm: int -> n:nat{n >= 2} -> Tot (x:int{x >= -(n/2) /\ x <= n/2})
 let mod_pm a n =
-  let res:nat = a % n in
+  let res = a % n in
   if res <= n/2 
   then res 
   else res - n
@@ -557,7 +550,7 @@ let intL n =
   mod_pm n (pow2 params_d)
   
 // mod_pm: R_q x Z -> R_q
-val poly_mod_pm: f:poly_t -> n:nat{n >= 2} -> Tot poly_t
+val poly_mod_pm: poly_t -> n:nat{n >= 2} -> poly_t
 let poly_mod_pm f n =
   repeati (Seq.length f)
   (fun i (f:poly_t) ->
@@ -568,15 +561,14 @@ let fnL f =
   assert_norm(pow2 params_d >= 2);
   poly_mod_pm f (pow2 params_d)
 
-// [*]_M: Z -> Z
 #reset-options "--z3rlimit 50 --max_fuel 0"
-val intM: c: int -> Tot field_t // (x:int{x > -params_q /\ x < params_q})
+
+// [*]_M: Z -> Z
+val intM: c: int -> field_t
 let intM c = 
-  assert_norm((pow2 params_d) >= 2);
+  assert_norm(pow2 params_d >= 2);
   let res = ((c `mod_pm` params_q) - (c `mod_pm` (pow2 params_d))) / (pow2 params_d) in
-  assume(res > -params_q); // TODO: Above line fails with --max-fuel 0 and goes off into the weeds without it, on the qTESLA-p-III parameter set.
   res
-  
 
 // [*]_M: R_q -> R_q
 val fnM: f: poly_t -> Tot poly_t
@@ -654,7 +646,15 @@ let rec qtesla_sign_step4 #mLen m sk r rand counter fuel =
        then qtesla_sign_step4 m sk r rand (add_mod counter (u16 1)) (fuel - 1)
        else Some (z, cPrime)
 
-assume val qtesla_sign_oracle:  #mLen: size_nat{params_k * params_n + mLen <= max_size_t} -> m: (lbytes mLen) -> sk: qtesla_sk -> r: (lbytes params_kappa) -> rand: (lbytes params_kappa) -> counter:uint16 -> Tot (fuel:nat{Some? (qtesla_sign_step4 #mLen m sk r rand counter fuel)})
+assume 
+val qtesla_sign_oracle: 
+    #mLen: size_nat{params_k * params_n + mLen <= max_size_t} 
+  -> m: (lbytes mLen) 
+  -> sk: qtesla_sk 
+  -> r: (lbytes params_kappa) 
+  -> rand: (lbytes params_kappa) 
+  -> counter:uint16 
+  -> Tot (fuel:nat{Some? (qtesla_sign_step4 #mLen m sk r rand counter fuel)})
 
 val qtesla_sign: #mLen: size_nat{params_k * params_n + mLen <= max_size_t} -> m: (lbytes mLen) -> sk: qtesla_sk -> Tot qtesla_sig
 let qtesla_sign #mLen m sk =
@@ -667,9 +667,14 @@ let qtesla_sign #mLen m sk =
   Some?.v res
 
 let compare (#len:size_nat) (test_expected:lbytes len) (test_result:lbytes len) =
-  for_all2 (fun a b -> uint_to_nat #U8 a = uint_to_nat #U8 b) test_expected test_result
+  lbytes_eq test_expected test_result
 
-val qtesla_verify: #mLen: size_nat{params_k * params_n + mLen <= max_size_t} -> m: (lbytes mLen) -> sig: qtesla_sig -> pk: qtesla_pk -> Tot bool
+val qtesla_verify: 
+    #mLen: size_nat{params_k * params_n + mLen <= max_size_t} 
+  -> m: (lbytes mLen) 
+  -> sig: qtesla_sig 
+  -> pk: qtesla_pk 
+  -> bool
 let qtesla_verify #mLen m sig pk =
   let z, cPrime = sig in
   let seedA, t = pk in
