qtesla/spec/params-qTesla-I/QTesla.Params.fst
@@ -1,0 +1,27 @@
+module QTesla.Params
+
+open Lib.IntTypes
+
+let params_lambda = 95 // security parameter
+let params_kappa = 32 // output length of hash function in bytes (spec lists them in bits, so convert)
+let params_n = 512 // Dimension
+let params_k = 1       // #R-LWE samples (number of polynomials in e, t, a, etc)
+let params_q = 4205569 // modulus
+let params_h = 30      // # of nonzero entries of output elements of Enc
+let params_Le = 1586   // bound on e_i for checkE
+let params_Ls = 1586   // bound on s for checkS
+let params_B = 1048575 // interval the randomness is chosing from during signing
+let params_d = 21      // number of rounded bits
+let params_bGenA = 19  // number of blocks requested to SHAKE128 for GenA
+
+let params_rateXOF = 168
+let params_xof = Spec.SHA3.shake128        // extendable output function used in PRF1: use shake128 or shake256 depending on parameters chosen
+let params_hash_shake = Spec.SHA3.shake128 // hash function used in hash H: use shake128 or shake256 depending on parameters chosen
+
+// See the GenerateNTTConstants-Magma.txt script for computing these five
+// constants used in NTT.
+let computed_phi = 3768668
+let computed_omega = 118029
+let computed_phi_inv = 3764481
+let computed_omega_inv = 590666
+let computed_n_inv = 4197355
